tuned structure and whitespace, augmenting some omissions on-the-fly at best guess

thys/Native_Word/Native_Word_Test.thy
@@ -4,7 +4,8 @@
 
 chapter \<open>Test cases\<close>
 
-theory Native_Word_Test imports
+theory Native_Word_Test
+imports
   Uint64 Uint32 Uint16 Uint8 Uint Native_Cast_Uint
   "HOL-Library.Code_Test" "Word_Lib.Bit_Shifts_Infix_Syntax"
 begin
@@ -23,8 +24,8 @@ context
   includes bit_operations_syntax
 begin
 
-definition bit_integer_test :: "bool" where
-  "bit_integer_test =
+definition bit_integer_test :: bool
+  where \<open>bit_integer_test =
   (([ -1 AND 3, 1 AND -3, 3 AND 5, -3 AND (- 5)
     , -3 OR 1, 1 OR -3, 3 OR 5, -3 OR (- 5)
     , NOT 1, NOT (- 3)
@@ -44,202 +45,37 @@ definition bit_integer_test :: "bool" where
       msb (5 :: integer), msb (0 :: integer), msb (-1 :: integer), msb (-2 :: integer)]
   = [ False, True, True, False,
       True, False, True, False,
-      False, False, True, True])"
+      False, False, True, True])\<close>
 
-export_code bit_integer_test checking SML Haskell? Haskell_Quickcheck? OCaml? Scala
+export_code bit_integer_test
+  checking SML Haskell? Haskell_Quickcheck? OCaml? Scala
 
-notepad begin
-have bit_integer_test by eval
-have bit_integer_test by normalization
-have bit_integer_test by code_simp
+notepad
+begin
+  have bit_integer_test by eval
+  have bit_integer_test by normalization
+  have bit_integer_test by code_simp
 end
+
 ML_val \<open>val true = @{code bit_integer_test}\<close>
 
-lemma "x AND y = x OR (y :: integer)"
-quickcheck[random, expect=counterexample]
-quickcheck[exhaustive, expect=counterexample]
+lemma \<open>x AND y = x OR (y :: integer)\<close>
+quickcheck [random, expect=counterexample]
+quickcheck [exhaustive, expect=counterexample]
 oops
 
-lemma "(x :: integer) AND x = x OR x"
-quickcheck[narrowing, expect=no_counterexample]
-oops
-
-lemma "(f :: integer \<Rightarrow> unit) = g"
-quickcheck[narrowing, size=3, expect=no_counterexample]
-by(simp add: fun_eq_iff)
-
-end
-
-hide_const bit_integer_test
-hide_fact bit_integer_test_def
-
-
-section \<open>Tests for @{typ uint32}\<close>
-
-context
-  includes bit_operations_syntax
-begin
-
-abbreviation (input) sshiftr_uint32 (infixl ">>>" 55)
-  where \<open>w >>> n \<equiv> signed_drop_bit_uint32 n w\<close>
-
-definition test_uint32 where
-  "test_uint32 \<longleftrightarrow>
-  (([ 0x100000001, -1, -4294967291, 0xFFFFFFFF, 0x12345678
-    , 0x5A AND 0x36
-    , 0x5A OR 0x36
-    , 0x5A XOR 0x36
-    , NOT 0x5A
-    , 5 + 6, -5 + 6, -6 + 5, -5 + (- 6), 0xFFFFFFFFF + 1
-    , 5 - 3, 3 - 5
-    , 5 * 3, -5 * 3, -5 * -4, 0x12345678 * 0x87654321
-    , 5 div 3, -5 div 3, -5 div -3, 5 div -3
-    , 5 mod 3, -5 mod 3, -5 mod -3, 5 mod -3
-    , set_bit 5 4 True, set_bit (- 5) 2 True, set_bit 5 0 False, set_bit (- 5) 1 False
-    , set_bit 5 32 True, set_bit 5 32 False, set_bit (- 5) 32 True, set_bit (- 5) 32 False
-    , 1 << 2, -1 << 3, 1 << 32, 1 << 0
-    , 100 >> 3, -100 >> 3, 100 >> 32, -100 >> 32
-    , 100 >>> 3, -100 >>> 3, 100 >>> 32, -100 >>> 32] :: uint32 list)
-   =
-    [ 1, 4294967295, 5, 4294967295, 305419896
-    , 18
-    , 126
-    , 108
-    , 4294967205
-    , 11, 1, 4294967295, 4294967285, 0
-    , 2, 4294967294
-    , 15, 4294967281, 20, 1891143032
-    , 1, 1431655763, 0, 0
-    , 2, 2, 4294967291, 5 
-    , 21, 4294967295, 4, 4294967289
-    , 5, 5, 4294967291, 4294967291
-    , 4, 4294967288, 0, 1
-    , 12, 536870899, 0, 0
-    , 12, 4294967283, 0, 4294967295]) \<and>
-  ([ (0x5 :: uint32) = 0x5, (0x5 :: uint32) = 0x6
-   , (0x5 :: uint32) < 0x5, (0x5 :: uint32) < 0x6, (-5 :: uint32) < 6, (6 :: uint32) < -5
-   , (0x5 :: uint32) \<le> 0x5, (0x5 :: uint32) \<le> 0x4, (-5 :: uint32) \<le> 6, (6 :: uint32) \<le> -5 
-   , (0x7FFFFFFF :: uint32) < 0x80000000, (0xFFFFFFFF :: uint32) < 0, (0x80000000 :: uint32) < 0x7FFFFFFF
-   , bit (0x7FFFFFFF :: uint32) 0, bit (0x7FFFFFFF :: uint32) 31, bit (0x80000000 :: uint32) 31, bit (0x80000000 :: uint32) 32
-   ]
-  =
-   [ True, False
-   , False, True, False, True
-   , True, False, False, True
-   , True, False, False
-   , True, False, True, False
-   ]) \<and>
-  ([integer_of_uint32 0, integer_of_uint32 0x7FFFFFFF, integer_of_uint32 0x80000000, integer_of_uint32 0xAAAAAAAA]
-  =
-   [0, 0x7FFFFFFF, 0x80000000, 0xAAAAAAAA])"
-
-export_code test_uint32 checking SML Haskell? OCaml? Scala
-
-notepad begin
-have test_uint32 by eval
-have test_uint32 by code_simp
-have test_uint32 by normalization
-end
-
-definition test_uint32' :: uint32 
-where "test_uint32' = 0 + 10 - 14 * 3 div 6 mod 3 << 3 >> 2"
-ML \<open>val 0wx12 = @{code test_uint32'}\<close>
-
-lemma "x AND y = x OR (y :: uint32)"
-quickcheck[random, expect=counterexample]
-quickcheck[exhaustive, expect=counterexample]
-oops
-
-lemma "(x :: uint32) AND x = x OR x"
-quickcheck[narrowing, expect=no_counterexample]
+lemma \<open>(x :: integer) AND x = x OR x\<close>
+quickcheck [narrowing, expect=no_counterexample]
 by transfer simp
 
-lemma "(f :: uint32 \<Rightarrow> unit) = g"
+lemma \<open>(f :: integer \<Rightarrow> unit) = g\<close>
 quickcheck[narrowing, size=3, expect=no_counterexample]
-by(simp add: fun_eq_iff)
+by (simp add: fun_eq_iff)
 
 end
 
 
-section \<open>Tests for @{typ uint16}\<close>
-
-context
-  includes bit_operations_syntax
-begin
-
-abbreviation (input) sshiftr_uint16 (infixl ">>>" 55)
-  where \<open>w >>> n \<equiv> signed_drop_bit_uint16 n w\<close>
-
-definition test_uint16 where
-  "test_uint16 \<longleftrightarrow>
-  (([ 0x10001, -1, -65535, 0xFFFF, 0x1234
-    , 0x5A AND 0x36
-    , 0x5A OR 0x36
-    , 0x5A XOR 0x36
-    , NOT 0x5A
-    , 5 + 6, -5 + 6, -6 + 5, -5 + -6, 0xFFFF + 1
-    , 5 - 3, 3 - 5
-    , 5 * 3, -5 * 3, -5 * -4, 0x1234 * 0x8765
-    , 5 div 3, -5 div 3, -5 div -3, 5 div -3
-    , 5 mod 3, -5 mod 3, -5 mod -3, 5 mod -3
-    , set_bit 5 4 True, set_bit (- 5) 2 True, set_bit 5 0 False, set_bit (- 5) 1 False
-    , set_bit 5 32 True, set_bit 5 32 False, set_bit (- 5) 32 True, set_bit (- 5) 32 False
-    , 1 << 2, -1 << 3, 1 << 16, 1 << 0
-    , 100 >> 3, -100 >> 3, 100 >> 16, -100 >> 16
-    , 100 >>> 3, -100 >>> 3, 100 >>> 16, -100 >>> 16] :: uint16 list)
-   =
-    [ 1, 65535, 1, 65535, 4660
-    , 18
-    , 126
-    , 108
-    , 65445
-    , 11, 1, 65535, 65525, 0
-    , 2, 65534
-    , 15, 65521, 20, 39556
-    , 1, 21843, 0, 0
-    , 2, 2, 65531, 5
-    , 21, 65535, 4, 65529
-    , 5, 5, 65531, 65531
-    , 4, 65528, 0, 1
-    , 12, 8179, 0, 0
-    , 12, 65523, 0, 65535]) \<and>
-  ([ (0x5 :: uint16) = 0x5, (0x5 :: uint16) = 0x6
-   , (0x5 :: uint16) < 0x5, (0x5 :: uint16) < 0x6, (-5 :: uint16) < 6, (6 :: uint16) < -5
-   , (0x5 :: uint16) \<le> 0x5, (0x5 :: uint16) \<le> 0x4, (-5 :: uint16) \<le> 6, (6 :: uint16) \<le> -5 
-   , (0x7FFF :: uint16) < 0x8000, (0xFFFF :: uint16) < 0, (0x8000 :: uint16) < 0x7FFF
-   , bit (0x7FFF :: uint16) 0, bit (0x7FFF :: uint16) 15, bit (0x8000 :: uint16) 15, bit (0x8000 :: uint16) 16
-   ]
-  =
-   [ True, False
-   , False, True, False, True
-   , True, False, False, True
-   , True, False, False
-   , True, False, True, False
-   ]) \<and>
-  ([integer_of_uint16 0, integer_of_uint16 0x7FFF, integer_of_uint16 0x8000, integer_of_uint16 0xAAAA]
-  =
-   [0, 0x7FFF, 0x8000, 0xAAAA])"
-
-export_code test_uint16 checking Haskell? Scala
-export_code test_uint16 checking SML_word
-
-notepad begin
-have test_uint16 by code_simp
-have test_uint16 by normalization
-end
-
-lemma "(x :: uint16) AND x = x OR x"
-quickcheck[narrowing, expect=no_counterexample]
-by transfer simp
-
-lemma "(f :: uint16 \<Rightarrow> unit) = g"
-quickcheck[narrowing, size=3, expect=no_counterexample]
-by(simp add: fun_eq_iff)
-
-end
-
-
-section \<open>Tests for @{typ uint8}\<close>
+section \<open>Tests for \<^typ>\<open>uint8\<close>\<close>
 
 context
   includes bit_operations_syntax
@@ -248,8 +84,8 @@ begin
 abbreviation (input) sshiftr_uint8 (infixl ">>>" 55)
   where \<open>w >>> n \<equiv> signed_drop_bit_uint8 n w\<close>
 
-definition test_uint8 where
-  "test_uint8 \<longleftrightarrow> 
+definition test_uint8 :: bool
+  where \<open>test_uint8 \<longleftrightarrow>
   (([ 0x101, -1, -255, 0xFF, 0x12
     , 0x5A AND 0x36
     , 0x5A OR 0x36
@@ -283,7 +119,7 @@ definition test_uint8 where
     , 12, 243, 0, 255]) \<and>
   ([ (0x5 :: uint8) = 0x5, (0x5 :: uint8) = 0x6
    , (0x5 :: uint8) < 0x5, (0x5 :: uint8) < 0x6, (-5 :: uint8) < 6, (6 :: uint8) < -5
-   , (0x5 :: uint8) \<le> 0x5, (0x5 :: uint8) \<le> 0x4, (-5 :: uint8) \<le> 6, (6 :: uint8) \<le> -5 
+   , (0x5 :: uint8) \<le> 0x5, (0x5 :: uint8) \<le> 0x4, (-5 :: uint8) \<le> 6, (6 :: uint8) \<le> -5
    , (0x7F :: uint8) < 0x80, (0xFF :: uint8) < 0, (0x80 :: uint8) < 0x7F
    , bit (0x7F :: uint8) 0, bit (0x7F :: uint8) 7, bit (0x80 :: uint8) 7, bit (0x80 :: uint8) 8
    ]
@@ -296,130 +132,208 @@ definition test_uint8 where
    ]) \<and>
   ([integer_of_uint8 0, integer_of_uint8 0x7F, integer_of_uint8 0x80, integer_of_uint8 0xAA]
   =
-   [0, 0x7F, 0x80, 0xAA])"
+   [0, 0x7F, 0x80, 0xAA])\<close>
 
-export_code test_uint8 checking SML Haskell? Scala
+export_code test_uint8
+  checking SML Haskell? Scala
 
-notepad begin
-
-have test_uint8 by eval
-have test_uint8 by code_simp
-have test_uint8 by normalization
+notepad
+begin
+  have test_uint8 by eval
+  have test_uint8 by code_simp
+  have test_uint8 by normalization
 end
+
 ML_val \<open>val true = @{code test_uint8}\<close>
 
 definition test_uint8' :: uint8
-where "test_uint8' = 0 + 10 - 14 * 3 div 6 mod 3 << 3 >> 2"
+  where \<open>test_uint8' = 0 + 10 - 14 * 3 div 6 mod 3 << 3 >> 2\<close>
+
 ML \<open>val 0wx12 = @{code test_uint8'}\<close>
 
-lemma "x AND y = x OR (y :: uint8)"
-quickcheck[random, expect=counterexample]
-quickcheck[exhaustive, expect=counterexample]
+lemma \<open>x AND y = x OR (y :: uint8)\<close>
+quickcheck [random, expect=counterexample]
+quickcheck [exhaustive, expect=counterexample]
 oops
 
-lemma "(x :: uint8) AND x = x OR x"
-quickcheck[narrowing, expect=no_counterexample]
+lemma \<open>(x :: uint8) AND x = x OR x\<close>
+quickcheck [narrowing, expect=no_counterexample]
 by transfer simp
 
-lemma "(f :: uint8 \<Rightarrow> unit) = g"
-quickcheck[narrowing, size=3, expect=no_counterexample]
-by(simp add: fun_eq_iff)
+lemma \<open>(f :: uint8 \<Rightarrow> unit) = g\<close>
+quickcheck [narrowing, size=3, expect=no_counterexample]
+by (simp add: fun_eq_iff)
 
 
-section \<open>Tests for @{typ "uint"}\<close>
+section \<open>Tests for \<^typ>\<open>uint16\<close>\<close>
 
 context
   includes bit_operations_syntax
 begin
 
-abbreviation (input) sshiftr_uint (infixl ">>>" 55)
-  where \<open>w >>> n \<equiv> signed_drop_bit_uint n w\<close>
+abbreviation (input) sshiftr_uint16 (infixl ">>>" 55)
+  where \<open>w >>> n \<equiv> signed_drop_bit_uint16 n w\<close>
 
-definition "test_uint \<equiv> let 
-  test_list1 = (let
-      HS = uint_of_int (2 ^ (dflt_size - 1))
-    in
-      ([ HS + HS + 1, -1, -HS - HS + 5, HS + (HS - 1), 0x12
-      , 0x5A AND 0x36
-      , 0x5A OR 0x36
-      , 0x5A XOR 0x36
-      , NOT 0x5A
-      , 5 + 6, -5 + 6, -6 + 5, -5 + -6, HS + (HS - 1) + 1
-      , 5 - 3, 3 - 5
-      , 5 * 3, -5 * 3, -5 * -4, 0x12345678 * 0x87654321]
-    @ (if dflt_size > 4 then
-      [ 5 div 3, -5 div 3, -5 div -3, 5 div -3
-      , 5 mod 3, -5 mod 3, -5 mod -3, 5 mod -3
-      , set_bit 5 4 True, set_bit (- 5) 2 True, set_bit 5 0 False, set_bit (- 5) 1 False
-      , set_bit 5 dflt_size True, set_bit 5 dflt_size False, set_bit (- 5) dflt_size True, set_bit (- 5) dflt_size False
-      , 1 << 2, -1 << 3, push_bit dflt_size 1, 1 << 0
-      , 31 >> 3, -1 >> 3, 31 >> dflt_size, -1 >> dflt_size
-      , 15 >>> 2, -1 >>> 3, 15 >>> dflt_size, -1 >>> dflt_size]
-    else []) :: uint list));
-  
-  test_list2 = (let 
-      S = wivs_shift 
-    in 
-      ([ 1, -1, -S + 5, S - 1, 0x12
-      , 0x5A AND 0x36
-      , 0x5A OR 0x36
-      , 0x5A XOR 0x36
-      , NOT 0x5A
-      , 5 + 6, -5 + 6, -6 + 5, -5 + -6, 0
-      , 5 - 3, 3 - 5
-      , 5 * 3, -5 * 3, -5 * -4, 0x12345678 * 0x87654321]
-    @ (if dflt_size > 4 then
-      [ 5 div 3, (S - 5) div 3, (S - 5) div (S - 3), 5 div (S - 3)
-      , 5 mod 3, (S - 5) mod 3, (S - 5) mod (S - 3), 5 mod (S - 3)
-      , set_bit 5 4 True, -1, set_bit 5 0 False, -7
-      , 5, 5, -5, -5
-      , 4, -8, 0, 1
-      , 3, (S >> 3) - 1, 0, 0
-      , 3, (S >> 1) + (S >> 1) - 1, 0, -1] 
-    else []) :: int list));
-
-  test_list_c1 = (let
-      HS = uint_of_int ((2^(dflt_size - 1)))
-    in
-  [  (0x5 :: uint) = 0x5, (0x5 :: uint) = 0x6
-   , (0x5 :: uint) < 0x5, (0x5 :: uint) < 0x6, (-5 :: uint) < 6, (6 :: uint) < -5
-   , (0x5 :: uint) \<le> 0x5, (0x5 :: uint) \<le> 0x4, (-5 :: uint) \<le> 6, (6 :: uint) \<le> -5 
-   , (HS - 1) < HS, (HS + HS - 1) < 0, HS < HS - 1
-   , bit (HS - 1) 0, bit (HS - 1 :: uint) (dflt_size - 1), bit (HS :: uint) (dflt_size - 1), bit (HS :: uint) dflt_size
-   ]);
-
-  test_list_c2 =
-   [ True, False
-   , False, dflt_size\<ge>2, dflt_size=3, dflt_size\<noteq>3
-   , True, False, dflt_size=3, dflt_size\<noteq>3
-   , True, False, False
-   , dflt_size\<noteq>1, False, True, False
+definition test_uint16 :: bool
+  where \<open>test_uint16 \<longleftrightarrow>
+  (([ 0x10001, -1, -65535, 0xFFFF, 0x1234
+    , 0x5A AND 0x36
+    , 0x5A OR 0x36
+    , 0x5A XOR 0x36
+    , NOT 0x5A
+    , 5 + 6, -5 + 6, -6 + 5, -5 + -6, 0xFFFF + 1
+    , 5 - 3, 3 - 5
+    , 5 * 3, -5 * 3, -5 * -4, 0x1234 * 0x8765
+    , 5 div 3, -5 div 3, -5 div -3, 5 div -3
+    , 5 mod 3, -5 mod 3, -5 mod -3, 5 mod -3
+    , set_bit 5 4 True, set_bit (- 5) 2 True, set_bit 5 0 False, set_bit (- 5) 1 False
+    , set_bit 5 32 True, set_bit 5 32 False, set_bit (- 5) 32 True, set_bit (- 5) 32 False
+    , 1 << 2, -1 << 3, 1 << 16, 1 << 0
+    , 100 >> 3, -100 >> 3, 100 >> 16, -100 >> 16
+    , 100 >>> 3, -100 >>> 3, 100 >>> 16, -100 >>> 16] :: uint16 list)
+   =
+    [ 1, 65535, 1, 65535, 4660
+    , 18
+    , 126
+    , 108
+    , 65445
+    , 11, 1, 65535, 65525, 0
+    , 2, 65534
+    , 15, 65521, 20, 39556
+    , 1, 21843, 0, 0
+    , 2, 2, 65531, 5
+    , 21, 65535, 4, 65529
+    , 5, 5, 65531, 65531
+    , 4, 65528, 0, 1
+    , 12, 8179, 0, 0
+    , 12, 65523, 0, 65535]) \<and>
+  ([ (0x5 :: uint16) = 0x5, (0x5 :: uint16) = 0x6
+   , (0x5 :: uint16) < 0x5, (0x5 :: uint16) < 0x6, (-5 :: uint16) < 6, (6 :: uint16) < -5
+   , (0x5 :: uint16) \<le> 0x5, (0x5 :: uint16) \<le> 0x4, (-5 :: uint16) \<le> 6, (6 :: uint16) \<le> -5
+   , (0x7FFF :: uint16) < 0x8000, (0xFFFF :: uint16) < 0, (0x8000 :: uint16) < 0x7FFF
+   , bit (0x7FFF :: uint16) 0, bit (0x7FFF :: uint16) 15, bit (0x8000 :: uint16) 15, bit (0x8000 :: uint16) 16
    ]
-in
-  test_list1 = map uint_of_int test_list2
-\<and> test_list_c1 = test_list_c2"
+  =
+   [ True, False
+   , False, True, False, True
+   , True, False, False, True
+   , True, False, False
+   , True, False, True, False
+   ]) \<and>
+  ([integer_of_uint16 0, integer_of_uint16 0x7FFF, integer_of_uint16 0x8000, integer_of_uint16 0xAAAA]
+  =
+   [0, 0x7FFF, 0x8000, 0xAAAA])\<close>
 
-export_code test_uint checking SML Haskell? OCaml? Scala
+export_code test_uint16 checking Haskell? Scala
+export_code test_uint16 checking SML_word
 
-lemma "test_uint"
-quickcheck[exhaustive, expect=no_counterexample]
-oops \<comment> \<open>FIXME: prove correctness of test by reflective means (not yet supported)\<close>
+notepad begin
+  have test_uint16 by code_simp
+  have test_uint16 by normalization
+end
 
-lemma "x AND y = x OR (y :: uint)"
-quickcheck[random, expect=counterexample]
-quickcheck[exhaustive, expect=counterexample]
-oops
-
-lemma "(x :: uint) AND x = x OR x"
-quickcheck[narrowing, expect=no_counterexample]
+lemma \<open>(x :: uint16) AND x = x OR x\<close>
+quickcheck [narrowing, expect=no_counterexample]
 by transfer simp
 
-lemma "(f :: uint \<Rightarrow> unit) = g"
-quickcheck[narrowing, size=3, expect=no_counterexample]
-by(simp add: fun_eq_iff)
+lemma \<open>(f :: uint16 \<Rightarrow> unit) = g\<close>
+quickcheck [narrowing, size=3, expect=no_counterexample]
+by (simp add: fun_eq_iff)
+
+end
 
 
-section \<open>Tests for @{typ uint64} \<close>
+section \<open>Tests for \<^typ>\<open>uint32\<close>\<close>
+
+context
+  includes bit_operations_syntax
+begin
+
+abbreviation (input) sshiftr_uint32 (infixl ">>>" 55)
+  where \<open>w >>> n \<equiv> signed_drop_bit_uint32 n w\<close>
+
+definition test_uint32 :: bool
+  where \<open>test_uint32 \<longleftrightarrow>
+  (([ 0x100000001, -1, -4294967291, 0xFFFFFFFF, 0x12345678
+    , 0x5A AND 0x36
+    , 0x5A OR 0x36
+    , 0x5A XOR 0x36
+    , NOT 0x5A
+    , 5 + 6, -5 + 6, -6 + 5, -5 + (- 6), 0xFFFFFFFFF + 1
+    , 5 - 3, 3 - 5
+    , 5 * 3, -5 * 3, -5 * -4, 0x12345678 * 0x87654321
+    , 5 div 3, -5 div 3, -5 div -3, 5 div -3
+    , 5 mod 3, -5 mod 3, -5 mod -3, 5 mod -3
+    , set_bit 5 4 True, set_bit (- 5) 2 True, set_bit 5 0 False, set_bit (- 5) 1 False
+    , set_bit 5 32 True, set_bit 5 32 False, set_bit (- 5) 32 True, set_bit (- 5) 32 False
+    , 1 << 2, -1 << 3, 1 << 32, 1 << 0
+    , 100 >> 3, -100 >> 3, 100 >> 32, -100 >> 32
+    , 100 >>> 3, -100 >>> 3, 100 >>> 32, -100 >>> 32] :: uint32 list)
+   =
+    [ 1, 4294967295, 5, 4294967295, 305419896
+    , 18
+    , 126
+    , 108
+    , 4294967205
+    , 11, 1, 4294967295, 4294967285, 0
+    , 2, 4294967294
+    , 15, 4294967281, 20, 1891143032
+    , 1, 1431655763, 0, 0
+    , 2, 2, 4294967291, 5 
+    , 21, 4294967295, 4, 4294967289
+    , 5, 5, 4294967291, 4294967291
+    , 4, 4294967288, 0, 1
+    , 12, 536870899, 0, 0
+    , 12, 4294967283, 0, 4294967295]) \<and>
+  ([ (0x5 :: uint32) = 0x5, (0x5 :: uint32) = 0x6
+   , (0x5 :: uint32) < 0x5, (0x5 :: uint32) < 0x6, (-5 :: uint32) < 6, (6 :: uint32) < -5
+   , (0x5 :: uint32) \<le> 0x5, (0x5 :: uint32) \<le> 0x4, (-5 :: uint32) \<le> 6, (6 :: uint32) \<le> -5
+   , (0x7FFFFFFF :: uint32) < 0x80000000, (0xFFFFFFFF :: uint32) < 0, (0x80000000 :: uint32) < 0x7FFFFFFF
+   , bit (0x7FFFFFFF :: uint32) 0, bit (0x7FFFFFFF :: uint32) 31, bit (0x80000000 :: uint32) 31, bit (0x80000000 :: uint32) 32
+   ]
+  =
+   [ True, False
+   , False, True, False, True
+   , True, False, False, True
+   , True, False, False
+   , True, False, True, False
+   ]) \<and>
+  ([integer_of_uint32 0, integer_of_uint32 0x7FFFFFFF, integer_of_uint32 0x80000000, integer_of_uint32 0xAAAAAAAA]
+  =
+   [0, 0x7FFFFFFF, 0x80000000, 0xAAAAAAAA])\<close>
+
+export_code test_uint32 checking SML Haskell? OCaml? Scala
+
+notepad begin
+  have test_uint32 by eval
+  have test_uint32 by code_simp
+  have test_uint32 by normalization
+end
+
+ML_val \<open>val true = @{code test_uint32}\<close>
+
+definition test_uint32' :: uint32 
+  where \<open>test_uint32' = 0 + 10 - 14 * 3 div 6 mod 3 << 3 >> 2\<close>
+
+ML \<open>val 0wx12 = @{code test_uint32'}\<close>
+
+lemma "x AND y = x OR (y :: uint32)"
+quickcheck [random, expect=counterexample]
+quickcheck [exhaustive, expect=counterexample]
+oops
+
+lemma "(x :: uint32) AND x = x OR x"
+quickcheck [narrowing, expect=no_counterexample]
+by transfer simp
+
+lemma "(f :: uint32 \<Rightarrow> unit) = g"
+quickcheck [narrowing, size=3, expect=no_counterexample]
+by (simp add: fun_eq_iff)
+
+end
+
+
+section \<open>Tests for \<^typ>\<open>uint64\<close> \<close>
 
 context
   includes bit_operations_syntax
@@ -428,8 +342,8 @@ begin
 abbreviation (input) sshiftr_uint64 (infixl ">>>" 55)
   where \<open>w >>> n \<equiv> signed_drop_bit_uint64 n w\<close>
 
-definition test_uint64 where
-  "test_uint64 \<longleftrightarrow>
+definition test_uint64 :: bool
+  where \<open>test_uint64 \<longleftrightarrow>
   (([ 0x10000000000000001, -1, -9223372036854775808, 0xFFFFFFFFFFFFFFFF, 0x1234567890ABCDEF
     , 0x5A AND 0x36
     , 0x5A OR 0x36
@@ -476,9 +390,9 @@ definition test_uint64 where
    ]) \<and>
   ([integer_of_uint64 0, integer_of_uint64 0x7FFFFFFFFFFFFFFF, integer_of_uint64 0x8000000000000000, integer_of_uint64 0xAAAAAAAAAAAAAAAA]
   =
-   [0, 0x7FFFFFFFFFFFFFFF, 0x8000000000000000, 0xAAAAAAAAAAAAAAAA])"
+   [0, 0x7FFFFFFFFFFFFFFF, 0x8000000000000000, 0xAAAAAAAAAAAAAAAA])\<close>
 
-value [nbe] "[0x10000000000000001, -1, -9223372036854775808, 0xFFFFFFFFFFFFFFFF, 0x1234567890ABCDEF
+value [nbe] \<open>[0x10000000000000001, -1, -9223372036854775808, 0xFFFFFFFFFFFFFFFF, 0x1234567890ABCDEF
     , 0x5A AND 0x36
     , 0x5A OR 0x36
     , 0x5A XOR 0x36
@@ -492,45 +406,142 @@ value [nbe] "[0x10000000000000001, -1, -9223372036854775808, 0xFFFFFFFFFFFFFFFF,
     , set_bit 5 64 True, set_bit 5 64 False, set_bit (- 5) 64 True, set_bit (- 5) 64 False
     , 1 << 2, -1 << 3, 1 << 64, 1 << 0
     , 100 >> 3, -100 >> 3, 100 >> 64, -100 >> 64
-    , 100 >>> 3, -100 >>> 3, 100 >>> 64, -100 >>> 64] :: uint64 list"
+    , 100 >>> 3, -100 >>> 3, 100 >>> 64, -100 >>> 64] :: uint64 list\<close>
 
 export_code test_uint64 checking SML Haskell? OCaml? Scala
 
 notepad begin
-have test_uint64 by eval
-have test_uint64 by code_simp
-have test_uint64 by normalization
+  have test_uint64 by eval
+  have test_uint64 by code_simp
+  have test_uint64 by normalization
 end
+
 ML_val \<open>val true = @{code test_uint64}\<close>
 
 definition test_uint64' :: uint64
-where "test_uint64' = 0 + 10 - 14 * 3 div 6 mod 3 << 3 >> 2"
+  where \<open>test_uint64' = 0 + 10 - 14 * 3 div 6 mod 3 << 3 >> 2\<close>
+
+ML \<open>val 0wx12 = @{code test_uint64'}\<close>
 
 end
+
+
+section \<open>Tests for \<^typ>\<open>uint\<close>\<close>
+
+context
+  includes bit_operations_syntax
+begin
+
+abbreviation (input) sshiftr_uint (infixl ">>>" 55)
+  where \<open>w >>> n \<equiv> signed_drop_bit_uint n w\<close>
+
+definition test_uint :: bool
+  where \<open>test_uint = (let
+  test_list1 = (let
+      HS = uint_of_int (2 ^ (dflt_size - 1))
+    in
+      ([ HS + HS + 1, -1, -HS - HS + 5, HS + (HS - 1), 0x12
+      , 0x5A AND 0x36
+      , 0x5A OR 0x36
+      , 0x5A XOR 0x36
+      , NOT 0x5A
+      , 5 + 6, -5 + 6, -6 + 5, -5 + -6, HS + (HS - 1) + 1
+      , 5 - 3, 3 - 5
+      , 5 * 3, -5 * 3, -5 * -4, 0x12345678 * 0x87654321]
+    @ (if dflt_size > 4 then
+      [ 5 div 3, -5 div 3, -5 div -3, 5 div -3
+      , 5 mod 3, -5 mod 3, -5 mod -3, 5 mod -3
+      , set_bit 5 4 True, set_bit (- 5) 2 True, set_bit 5 0 False, set_bit (- 5) 1 False
+      , set_bit 5 dflt_size True, set_bit 5 dflt_size False, set_bit (- 5) dflt_size True, set_bit (- 5) dflt_size False
+      , 1 << 2, -1 << 3, push_bit dflt_size 1, 1 << 0
+      , 31 >> 3, -1 >> 3, 31 >> dflt_size, -1 >> dflt_size
+      , 15 >>> 2, -1 >>> 3, 15 >>> dflt_size, -1 >>> dflt_size]
+    else []) :: uint list));
+
+  test_list2 = (let
+      S = wivs_shift
+    in
+      ([ 1, -1, -S + 5, S - 1, 0x12
+      , 0x5A AND 0x36
+      , 0x5A OR 0x36
+      , 0x5A XOR 0x36
+      , NOT 0x5A
+      , 5 + 6, -5 + 6, -6 + 5, -5 + -6, 0
+      , 5 - 3, 3 - 5
+      , 5 * 3, -5 * 3, -5 * -4, 0x12345678 * 0x87654321]
+    @ (if dflt_size > 4 then
+      [ 5 div 3, (S - 5) div 3, (S - 5) div (S - 3), 5 div (S - 3)
+      , 5 mod 3, (S - 5) mod 3, (S - 5) mod (S - 3), 5 mod (S - 3)
+      , set_bit 5 4 True, -1, set_bit 5 0 False, -7
+      , 5, 5, -5, -5
+      , 4, -8, 0, 1
+      , 3, (S >> 3) - 1, 0, 0
+      , 3, (S >> 1) + (S >> 1) - 1, 0, -1]
+    else []) :: int list));
+
+  test_list_c1 = (let
+      HS = uint_of_int ((2^(dflt_size - 1)))
+    in
+  [  (0x5 :: uint) = 0x5, (0x5 :: uint) = 0x6
+   , (0x5 :: uint) < 0x5, (0x5 :: uint) < 0x6, (-5 :: uint) < 6, (6 :: uint) < -5
+   , (0x5 :: uint) \<le> 0x5, (0x5 :: uint) \<le> 0x4, (-5 :: uint) \<le> 6, (6 :: uint) \<le> -5
+   , (HS - 1) < HS, (HS + HS - 1) < 0, HS < HS - 1
+   , bit (HS - 1) 0, bit (HS - 1 :: uint) (dflt_size - 1), bit (HS :: uint) (dflt_size - 1), bit (HS :: uint) dflt_size
+   ]);
+
+  test_list_c2 =
+   [ True, False
+   , False, dflt_size\<ge>2, dflt_size=3, dflt_size\<noteq>3
+   , True, False, dflt_size=3, dflt_size\<noteq>3
+   , True, False, False
+   , dflt_size\<noteq>1, False, True, False
+   ]
+in
+  test_list1 = map uint_of_int test_list2
+\<and> test_list_c1 = test_list_c2)\<close>
+
+export_code test_uint checking SML Haskell? OCaml? Scala
+
+lemma test_uint
+quickcheck[exhaustive, expect=no_counterexample]
+oops \<comment> \<open>FIXME: prove correctness of test by reflective means (not yet supported)\<close>
+
+lemma \<open>x AND y = x OR (y :: uint)\<close>
+quickcheck [random, expect=counterexample]
+quickcheck [exhaustive, expect=counterexample]
+oops
+
+lemma \<open>(x :: uint) AND x = x OR x\<close>
+quickcheck [narrowing, expect=no_counterexample]
+by transfer simp
+
+lemma \<open>(f :: uint \<Rightarrow> unit) = g\<close>
+quickcheck [narrowing, size=3, expect=no_counterexample]
+by (simp add: fun_eq_iff)
 
 
 section \<open>Tests for casts\<close>
 
 definition test_casts :: bool
-where "test_casts \<longleftrightarrow>
+  where \<open>test_casts \<longleftrightarrow>
   map uint8_of_uint32 [10, 0, 0xFE, 0xFFFFFFFF] = [10, 0, 0xFE, 0xFF] \<and>
   map uint8_of_uint64 [10, 0, 0xFE, 0xFFFFFFFFFFFFFFFF] = [10, 0, 0xFE, 0xFF] \<and>
   map uint32_of_uint8 [10, 0, 0xFF] = [10, 0, 0xFF] \<and>
-  map uint64_of_uint8 [10, 0, 0xFF] = [10, 0, 0xFF]"
+  map uint64_of_uint8 [10, 0, 0xFF] = [10, 0, 0xFF]\<close>
 
 definition test_casts' :: bool
-where "test_casts' \<longleftrightarrow>
+  where \<open>test_casts' \<longleftrightarrow>
   map uint8_of_uint16 [10, 0, 0xFE, 0xFFFF] = [10, 0, 0xFE, 0xFF] \<and>
   map uint16_of_uint8 [10, 0, 0xFF] = [10, 0, 0xFF] \<and>
   map uint16_of_uint32 [10, 0, 0xFFFE, 0xFFFFFFFF] = [10, 0, 0xFFFE, 0xFFFF] \<and>
   map uint16_of_uint64 [10, 0, 0xFFFE, 0xFFFFFFFFFFFFFFFF] = [10, 0, 0xFFFE, 0xFFFF] \<and>
   map uint32_of_uint16 [10, 0, 0xFFFF] = [10, 0, 0xFFFF] \<and>
-  map uint64_of_uint16 [10, 0, 0xFFFF] = [10, 0, 0xFFFF]"
+  map uint64_of_uint16 [10, 0, 0xFFFF] = [10, 0, 0xFFFF]\<close>
 
 definition test_casts'' :: bool
-where "test_casts'' \<longleftrightarrow>
+  where \<open>test_casts'' \<longleftrightarrow>
   map uint32_of_uint64 [10, 0, 0xFFFFFFFE, 0xFFFFFFFFFFFFFFFF] = [10, 0, 0xFFFFFFFE, 0xFFFFFFFF] \<and>
-  map uint64_of_uint32 [10, 0, 0xFFFFFFFF] = [10, 0, 0xFFFFFFFF]"
+  map uint64_of_uint32 [10, 0, 0xFFFFFFFF] = [10, 0, 0xFFFFFFFF]\<close>
 
 export_code test_casts test_casts'' checking SML Haskell? Scala
 export_code test_casts'' checking OCaml?
@@ -546,13 +557,14 @@ notepad begin
   have test_casts'' by normalization
   have test_casts'' by code_simp
 end
+
 ML \<open>
   val true = @{code test_casts}
   val true = @{code test_casts''}
 \<close>
 
-definition test_casts_uint :: bool where
-  "test_casts_uint \<longleftrightarrow>
+definition test_casts_uint :: bool
+  where \<open>test_casts_uint \<longleftrightarrow>
   map uint_of_uint32 ([0, 10] @ (if dflt_size < 32 then [push_bit (dflt_size - 1) 1, 0xFFFFFFFF] else [0xFFFFFFFF])) = 
   [0, 10] @ (if dflt_size < 32 then [push_bit (dflt_size - 1) 1, (push_bit dflt_size 1) - 1] else [0xFFFFFFFF]) \<and>
   map uint32_of_uint [0, 10, if dflt_size < 32 then push_bit (dflt_size - 1) 1 else 0xFFFFFFFF] =
@@ -560,17 +572,21 @@ definition test_casts_uint :: bool where
   map uint_of_uint64 [0, 10, push_bit (dflt_size - 1) 1, 0xFFFFFFFFFFFFFFFF] =
   [0, 10, push_bit (dflt_size - 1) 1, (push_bit dflt_size 1) - 1] \<and>
   map uint64_of_uint [0, 10, push_bit (dflt_size - 1) 1] =
-  [0, 10, push_bit (dflt_size - 1) 1]"
+  [0, 10, push_bit (dflt_size - 1) 1]\<close>
 
-definition test_casts_uint' :: bool where
-  "test_casts_uint' \<longleftrightarrow>
+definition test_casts_uint' :: bool
+  where \<open>test_casts_uint' \<longleftrightarrow>
   map uint_of_uint16 [0, 10, 0xFFFF] = [0, 10, 0xFFFF] \<and>
-  map uint16_of_uint [0, 10, 0xFFFF] = [0, 10, 0xFFFF]"
+  map uint16_of_uint [0, 10, 0xFFFF] = [0, 10, 0xFFFF]\<close>
 
-definition test_casts_uint'' :: bool where
-  "test_casts_uint'' \<longleftrightarrow>
+definition test_casts_uint'' :: bool
+  where \<open>test_casts_uint'' \<longleftrightarrow>
   map uint_of_uint8 [0, 10, 0xFF] = [0, 10, 0xFF] \<and>
-  map uint8_of_uint [0, 10, 0xFF] = [0, 10, 0xFF]"
+  map uint8_of_uint [0, 10, 0xFF] = [0, 10, 0xFF]\<close>
+
+export_code test_casts_uint test_casts_uint'' checking SML Haskell?
+export_code test_casts_uint checking OCaml?
+export_code test_casts_uint' checking Haskell? Scala
 
 end
 
