thys/Native_Word/Native_Word_Test_Emu.thy
@@ -2,31 +2,46 @@
     Author:     Andreas Lochbihler, ETH Zurich
 *)
 
-theory Native_Word_Test_Emu imports
+theory Native_Word_Test_Emu
+  imports
   Native_Word_Test
   Code_Target_Int_Bit
 begin
 
 section \<open>Test cases for emulation of native words\<close>
 
-subsection \<open>Tests for @{typ uint16}\<close>
+subsection \<open>Tests for \<^typ>\<open>uint8\<close>\<close>
 
 text \<open>
-  Test that @{typ uint16} is emulated for PolyML and OCaml via @{typ "16 word"} 
-  if @{theory Native_Word.Code_Target_Int_Bit} is imported.
+  Test that \<^typ>\<open>uint8\<close> is emulated for OCaml via \<^typ>\<open>8 word\<close>
+  if \<^theory>\<open>Native_Word.Code_Target_Int_Bit\<close> is imported.
 \<close>
 
-definition test_uint16_emulation :: bool where
-  "test_uint16_emulation \<longleftrightarrow> (0xFFFFF - 0x1000 = (0xEFFF :: uint16))"
+definition test_uint8_emulation :: bool
+  where \<open>test_uint8_emulation \<longleftrightarrow> (0xFFF - 0x10 = (0xEF :: uint8))\<close>
+
+export_code test_uint8_emulation checking OCaml?
+  \<comment> \<open>test the other target languages as well\<close> SML Haskell? Scala
+
+
+subsection \<open>Tests for \<^typ>\<open>uint16\<close>\<close>
+
+text \<open>
+  Test that \<^typ>\<open>uint16\<close> is emulated for PolyML and OCaml via \<^typ>\<open>16 word\<close>
+  if \<^theory>\<open>Native_Word.Code_Target_Int_Bit\<close> is imported.
+\<close>
+
+definition test_uint16_emulation :: bool
+  where \<open>test_uint16_emulation \<longleftrightarrow> (0xFFFFF - 0x1000 = (0xEFFF :: uint16))\<close>
 
 export_code test_uint16_emulation checking SML OCaml?
   \<comment> \<open>test the other target languages as well\<close> Haskell? Scala
 
 notepad begin
-have test_uint16 by eval
-have test_uint16_emulation by eval
-have test_uint16_emulation by normalization
-have test_uint16_emulation by code_simp
+  have test_uint16 by eval
+  have test_uint16_emulation by eval
+  have test_uint16_emulation by normalization
+  have test_uint16_emulation by code_simp
 end
 
 ML_val \<open>
@@ -34,22 +49,9 @@ ML_val \<open>
   val true = @{code test_uint16_emulation};
 \<close>
 
-lemma "x AND y = x OR (y :: uint16)"
-quickcheck[random, expect=counterexample]
-quickcheck[exhaustive, expect=counterexample]
+lemma \<open>x AND y = x OR (y :: uint16)\<close>
+quickcheck [random, expect=counterexample]
+quickcheck [exhaustive, expect=counterexample]
 oops
-
-subsection \<open>Tests for @{typ uint8}\<close>
-
-text \<open>
-  Test that @{typ uint8} is emulated for OCaml via @{typ "8 word"} 
-  if @{theory Native_Word.Code_Target_Int_Bit} is imported.
-\<close>
-
-definition test_uint8_emulation :: bool where
-  "test_uint8_emulation \<longleftrightarrow> (0xFFF - 0x10 = (0xEF :: uint8))"
-
-export_code test_uint8_emulation checking OCaml?
-  \<comment> \<open>test the other target languages as well\<close> SML Haskell? Scala
 
 end
