thys/Native_Word/Native_Word_Test_OCaml2.thy
@@ -2,13 +2,14 @@
     Author:     Andreas Lochbihler, ETH Zurich
 *)
 
-theory Native_Word_Test_OCaml2 imports
+theory Native_Word_Test_OCaml2
+  imports
   Native_Word_Test_Emu
 begin
 
 test_code
   test_uint16 test_uint16_emulation
-  test_uint8 "test_uint8' = 0x12" test_uint8_emulation
+  test_uint8 \<open>test_uint8' = 0x12\<close> test_uint8_emulation
   test_casts test_casts'
   test_casts_uint' test_casts_uint''
 in OCaml
