thys/Native_Word/Native_Word_Test_PolyML.thy
@@ -2,16 +2,17 @@
     Author:     Andreas Lochbihler, ETH Zurich
 *)
 
-theory Native_Word_Test_PolyML imports
+theory Native_Word_Test_PolyML
+imports
   Native_Word_Test
 begin
 
 section \<open>Test with PolyML\<close>
 
 test_code
-  test_uint64 "test_uint64' = 0x12"
-  test_uint32 "test_uint32' = 0x12"
-  test_uint8 "test_uint8' = 0x12"
+  test_uint64 \<open>test_uint64' = 0x12\<close>
+  test_uint32 \<open>test_uint32' = 0x12\<close>
+  test_uint8 \<open>test_uint8' = 0x12\<close>
   test_uint
   test_casts test_casts''
   test_casts_uint test_casts_uint''
