thys/Native_Word/Native_Word_Test_Scala.thy
@@ -2,24 +2,26 @@
     Author:     Andreas Lochbihler, ETH Zurich
 *)
 
-theory Native_Word_Test_Scala imports
+theory Native_Word_Test_Scala
+imports
   Native_Word_Test
 begin
 
 section \<open>Test with Scala\<close>
 
 text \<open>
-  In Scala, @{typ uint} and @{typ uint32} are both implemented as type \texttt{Int}.
+  In Scala, \<^typ>\<open>uint\<close> and\<^typ>\<open>uint32\<close> are both implemented as type \texttt{Int}.
   When they are used in the same generated program, we have to suppress the type class
   instances for one of them.
 \<close>
+
 code_printing class_instance uint32 :: equal \<rightharpoonup> (Scala) -
 
 test_code
-  test_uint64 "test_uint64' = 0x12"
-  test_uint32 "test_uint32' = 0x12"
+  test_uint64 \<open>test_uint64' = 0x12\<close>
+  test_uint32 \<open>test_uint32' = 0x12\<close>
   test_uint16
-  test_uint8 "test_uint8' = 0x12" 
+  test_uint8 \<open>test_uint8' = 0x12\<close>
   test_uint
   test_casts test_casts' test_casts''
   test_casts_uint test_casts_uint' test_casts_uint''
